lib/everparse/3d/EverParse3d.Actions.Base.fsti
@@ -1,1 +1,942 @@
 module EverParse3d.Actions.Base
+#lang-pulse
+open EverParse3d.ErrorCode
+open EverParse3d.Prelude
+open Pulse.Lib.Pervasives
+module I = EverParse3d.InputStream.Base
+module CP = EverParse3d.CopyBuffer
+module PA = EverParse3d.ProbeActions
+module AppCtxt = EverParse3d.AppCtxt
+open FStar.FunctionalExtensionality
+open EverParse3d.Actions.Common
+module U8 = FStar.UInt8
+module U32 = FStar.UInt32
+module U64 = FStar.UInt64
+module P = EverParse3d.Prelude
+module SZ = FStar.SizeT
+open EverParse3d.State
+module LP = LowParse.Spec.Base
+module FLD = LowParse.Spec.FLData
+module LPL = LowParse.Spec.List
+module LPP = LowParse.PulseParse.Base
+module LUT = LowParse.Spec.ListUpTo
+
+val action
+  (#base_t #len_t #pos_t: Type0)
+  {| inst: I.input_stream_inst base_t len_t pos_t  |}
+  (extra_state: state_dict)
+  (a: Type0)
+  (use_error_handler: bool)
+: Type0
+
+inline_for_extraction noextract
+val validate_with_action_t
+  (#base_t #len_t #pos_t: Type0)
+  {| inst: I.input_stream_inst base_t len_t pos_t  |}
+     (#nz:bool)
+     (#wk: _)
+     (#k:parser_kind nz wk)
+     (#t:Type0)
+     (p:parser k t)
+     (extra_state: state_dict)
+     (has_action:bool)
+     (use_error_handler:bool)
+: Type0
+
+inline_for_extraction noextract
+val validate_with_action_no_read
+  (#base_t #len_t #pos_t: Type0)
+  {| inst: I.input_stream_inst base_t len_t pos_t  |}
+     (#nz:bool)
+     (#wk: _)
+     (#k:parser_kind nz wk)
+     (#t:Type0)
+     (p:parser k t)
+     (extra_state: state_dict)
+     (has_action:bool)
+     (use_error_handler:bool)
+: Type0
+
+inline_for_extraction noextract
+val validate_eta
+  (#base_t #len_t #pos_t: Type0)
+  {| inst: I.input_stream_inst base_t len_t pos_t  |}
+      (#nz:bool)
+      (#wk: _)
+      (#k:parser_kind nz wk)
+      (#t:Type)
+      (#p:parser k t)
+      (#extra_state: state_dict)
+      (#has_action:bool)
+      (#use_error_handler:bool)
+      (v: validate_with_action_t #base_t #len_t #pos_t p extra_state has_action use_error_handler)
+: validate_with_action_t #base_t #len_t #pos_t p extra_state has_action use_error_handler
+
+inline_for_extraction noextract
+val act_with_comment
+  (#base_t #len_t #pos_t: Type0)
+  {| inst: I.input_stream_inst base_t len_t pos_t  |}
+      (s: string)
+      (extra_state: state_dict)
+      (#use_error_handler:bool)
+      (#res:Type)
+      (a: action #base_t #len_t #pos_t extra_state res use_error_handler)
+: action #base_t #len_t #pos_t extra_state res use_error_handler
+
+inline_for_extraction
+val leaf_reader
+  (#base_t #len_t #pos_t: Type0)
+  {| inst: I.input_stream_inst base_t len_t pos_t  |}
+  (#nz:bool)
+  (#k: parser_kind nz WeakKindStrongPrefix)
+  (#t: Type)
+  (p: parser k t)
+: Tot Type0
+
+inline_for_extraction noextract
+val validate_with_success_action
+  (#base_t #len_t #pos_t: Type0)
+  {| inst: I.input_stream_inst base_t len_t pos_t  |}
+      (name: string)
+      (#nz:bool)
+      (#wk: _)
+      (#k1:parser_kind nz wk)
+      (#t1:Type)
+      (#p1:parser k1 t1)
+      (#extra: state_dict)
+      (#has_action:bool)
+      (#use_error_handler:bool)
+      (v1:validate_with_action_t #base_t #len_t #pos_t p1 extra has_action use_error_handler)
+      (a:action #base_t #len_t #pos_t extra bool use_error_handler)
+  : validate_with_action_t #base_t #len_t #pos_t p1 extra true use_error_handler
+
+inline_for_extraction noextract
+val validate_with_error_handler
+  (#base_t #len_t #pos_t: Type0)
+  {| inst: I.input_stream_inst base_t len_t pos_t  |}
+  (error_handler_macro: error_handler #base_t #len_t #pos_t)
+      (typename: string)
+      (fieldname: string)
+      (#nz: _)
+      (#wk: _)
+      (#k1:parser_kind nz wk)
+      (#t1: Type)
+      (#p1:parser k1 t1)
+      (#extra_state: state_dict)
+      (#has_action: _)
+      (#use_error_handler:bool)
+      (v1:validate_with_action_t #base_t #len_t #pos_t p1 extra_state has_action use_error_handler)
+  : validate_with_action_t #base_t #len_t #pos_t p1 extra_state has_action use_error_handler
+
+inline_for_extraction noextract
+val validate_ret
+  (#base_t #len_t #pos_t: Type0)
+  {| inst: I.input_stream_inst base_t len_t pos_t  |}
+      (#extra_state: state_dict)
+      (#use_error_handler:bool)
+  : validate_with_action_t #base_t #len_t #pos_t (parse_ret ()) extra_state false use_error_handler
+
+inline_for_extraction noextract
+val validate_pair
+  (#base_t #len_t #pos_t: Type0)
+  {| inst: I.input_stream_inst base_t len_t pos_t  |}
+       (typename: string)
+       (name1: string)
+       (#nz1:_)
+       (#k1:parser_kind nz1 WeakKindStrongPrefix)
+       (#t1:Type)
+       (#p1:parser k1 t1)
+       (k1_const: bool)
+       (#extra_state: state_dict)
+       (#has_action1:bool)
+       (#use_error_handler:bool)
+       (v1:validate_with_action_t #base_t #len_t #pos_t p1 extra_state has_action1 use_error_handler)
+       (#nz2:_)
+       (#wk2: _)
+       (#k2:parser_kind nz2 wk2)
+       (#t2:Type)
+       (#p2:parser k2 t2)
+       (k2_const: bool)
+       (#has_action2:bool)
+       (v2:validate_with_action_t #base_t #len_t #pos_t p2 extra_state has_action2 use_error_handler)
+  : validate_with_action_t
+      #base_t #len_t #pos_t
+      (p1 `parse_pair` p2)
+      extra_state
+      (has_action1 || has_action2)
+      use_error_handler
+
+inline_for_extraction noextract
+val validate_dep_pair_with_refinement_and_action
+  (#base_t #len_t #pos_t: Type0)
+  {| inst: I.input_stream_inst base_t len_t pos_t  |}
+      (p1_is_constant_size_without_actions: bool)
+      (name1: string)
+      (#nz1:_)
+      (#k1:parser_kind nz1 WeakKindStrongPrefix)
+      (#t1:Type)
+      (#p1:parser k1 t1)
+      (#extra_state: state_dict)
+      (#has_action1:bool)
+      (#use_error_handler:bool)
+      (v1:validate_with_action_no_read #base_t #len_t #pos_t p1 extra_state has_action1 use_error_handler)
+      (r1: leaf_reader #base_t #len_t #pos_t p1)
+      (f: t1 -> bool)
+      (a:t1 -> action #base_t #len_t #pos_t extra_state bool use_error_handler)
+      (#nz2:_)
+      (#wk2: _)
+      (#k2:parser_kind nz2 wk2)
+      (#t2:refine _ f -> Type)
+      (#p2:(x:refine _ f -> parser k2 (t2 x)))
+      (#has_action2:bool)
+      (v2:(x:refine _ f -> validate_with_action_t #base_t #len_t #pos_t (p2 x) extra_state has_action2 use_error_handler))
+  : validate_with_action_t
+      #base_t #len_t #pos_t
+      ((p1 `parse_filter` f) `parse_dep_pair` p2)
+      extra_state
+      true
+      use_error_handler
+
+inline_for_extraction noextract
+val validate_filter
+  (#base_t #len_t #pos_t: Type0)
+  {| inst: I.input_stream_inst base_t len_t pos_t  |}
+       (name: string)
+       (#nz:_)
+       (#k:parser_kind nz WeakKindStrongPrefix)
+       (#t:Type)
+       (#p:parser k t)
+       (#extra_state: state_dict)
+       (#has_action:_)
+       (#use_error_handler:bool)
+       (v:validate_with_action_no_read #base_t #len_t #pos_t p extra_state has_action use_error_handler)
+       (r:leaf_reader #base_t #len_t #pos_t p)
+       (f:t -> bool)
+       (cr:string)
+       (cf:string)
+  : validate_with_action_t #base_t #len_t #pos_t (p `parse_filter` f) extra_state has_action use_error_handler
+
+inline_for_extraction noextract
+val validate_filter_with_action
+  (#base_t #len_t #pos_t: Type0)
+  {| inst: I.input_stream_inst base_t len_t pos_t  |}
+       (name: string)
+       (#nz:_)
+       (#k:parser_kind nz WeakKindStrongPrefix)
+       (#t:Type)
+       (#p:parser k t)
+       (#extra_state: state_dict)
+       (#has_action:_)
+       (#use_error_handler:bool)
+       (v:validate_with_action_no_read #base_t #len_t #pos_t p extra_state has_action use_error_handler)
+       (r:leaf_reader #base_t #len_t #pos_t p)
+       (f:t -> bool)
+       (cr:string)
+       (cf:string)
+       (a: t -> action #base_t #len_t #pos_t extra_state bool use_error_handler)
+  : validate_with_action_t
+      #base_t #len_t #pos_t
+      (p `parse_filter` f)
+      extra_state
+      true
+      use_error_handler
+
+inline_for_extraction noextract
+val validate_weaken_left
+  (#base_t #len_t #pos_t: Type0)
+  {| inst: I.input_stream_inst base_t len_t pos_t  |}
+       (#nz:_)
+       (#wk: _)
+       (#k:parser_kind nz wk)
+       (#t:Type)
+       (#p:parser k t)
+       (#extra_state: state_dict)
+       (#has_action:_)
+       (#use_error_handler:bool)
+       (v:validate_with_action_t #base_t #len_t #pos_t p extra_state has_action use_error_handler)
+       (#nz':_)
+       (#wk': _)
+       (k':parser_kind nz' wk')
+  : validate_with_action_t #base_t #len_t #pos_t (parse_weaken_left p k') extra_state has_action use_error_handler
+
+inline_for_extraction noextract
+val validate_weaken_right
+  (#base_t #len_t #pos_t: Type0)
+  {| inst: I.input_stream_inst base_t len_t pos_t  |}
+       (#nz:_)
+       (#wk: _)
+       (#k:parser_kind nz wk)
+       (#t:Type)
+       (#p:parser k t)
+       (#extra_state: state_dict)
+       (#has_action:_)
+       (#use_error_handler:bool)
+       (v:validate_with_action_t #base_t #len_t #pos_t p extra_state has_action use_error_handler)
+       (#nz':_)
+       (#wk': _)
+       (k':parser_kind nz' wk')
+  : validate_with_action_t #base_t #len_t #pos_t (parse_weaken_right p k') extra_state has_action use_error_handler
+
+noextract
+inline_for_extraction
+val validate_weaken
+  (#base_t #len_t #pos_t: Type0)
+  {| inst: I.input_stream_inst base_t len_t pos_t  |}
+       (name: string)
+       (#nz:_)
+       (#wk:_)
+       (#k:parser_kind nz wk)
+       (#t:Type)
+       (#p:parser k t)
+       (#d1: state_dict)
+       (#has_action:_)
+       (#use_error_handler:bool)
+       (v:validate_with_action_t #base_t #len_t #pos_t p d1 has_action use_error_handler)
+      (d2: state_dict)
+      (d2_extends: squash (state_dict_weaken_prop d1 d2))
+: validate_with_action_t #base_t #len_t #pos_t p d2 has_action use_error_handler
+
+noextract
+inline_for_extraction
+val validate_call
+  (#base_t #len_t #pos_t: Type0)
+  {| inst: I.input_stream_inst base_t len_t pos_t  |}
+       (name: string)
+       (#nz:_)
+       (#wk:_)
+       (#k:parser_kind nz wk)
+       (#t:Type)
+       (#p:parser k t)
+       (#d': state_dict)
+       (#has_action:_)
+       (#use_error_handler:bool)
+       (v:validate_with_action_t #base_t #len_t #pos_t p d' has_action use_error_handler)
+      (d: state_dict)
+      (#f: Ghost.erased ((x: refine_bool_t string d.state_p) -> Tot (option (refine_bool_t string d'.state_p)))) // TODO: change to GTot once we switch to ghost bijections
+      (#g: Ghost.erased (refine_bool_t string d'.state_p -> Tot (refine_bool_t string d.state_p)))
+      (sq: squash (state_dict_rename_prop d d' f g))
+: validate_with_action_t #base_t #len_t #pos_t p d has_action use_error_handler
+
+inline_for_extraction noextract
+val validate_impos
+  (#base_t #len_t #pos_t: Type0)
+  {| inst: I.input_stream_inst base_t len_t pos_t  |}
+       (#extra_state: _)
+       (#use_error_handler:bool)
+       (_:unit)
+  : validate_with_action_t #base_t #len_t #pos_t (parse_impos ()) extra_state false use_error_handler
+
+noextract inline_for_extraction
+val validate_ite
+  (#base_t #len_t #pos_t: Type0)
+  {| inst: I.input_stream_inst base_t len_t pos_t  |}
+       (#nz:_)
+       (#wk: _)
+       (#k:parser_kind nz wk)
+       (e:bool)
+       (#a:squash e -> Type)
+       (#b:squash (not e) -> Type)
+       (#extra_state: _)
+       (#ha1:_)
+       (#ha2:_)
+       (#use_error_handler:bool)
+       (p1:squash e -> parser k (a()))
+       (v1:(squash e -> validate_with_action_t #base_t #len_t #pos_t (p1()) extra_state ha1 use_error_handler))
+       (p2:squash (not e) -> parser k (b()))
+       (v2:(squash (not e) -> validate_with_action_t #base_t #len_t #pos_t (p2()) extra_state ha2 use_error_handler))
+  : validate_with_action_t
+      #base_t #len_t #pos_t
+      (parse_ite e p1 p2)
+      extra_state
+      (ha1 || ha2)
+      use_error_handler
+
+noextract inline_for_extraction
+val validate_nlist
+  (#base_t #len_t #pos_t: Type0)
+  {| inst: I.input_stream_inst base_t len_t pos_t  |}
+       (n:U32.t)
+       (n_is_const:option nat { memoizes_n_as_const n_is_const n})
+       (#wk: _)
+       (#k:parser_kind true wk)
+       (#t:Type)
+       (#p:parser k t)
+       (#extra_state: _)
+       (#ha:bool)
+       (#use_error_handler:bool)
+       (v: validate_with_action_t #base_t #len_t #pos_t p extra_state ha use_error_handler)
+: validate_with_action_t #base_t #len_t #pos_t (parse_nlist n n_is_const p) extra_state ha use_error_handler
+
+noextract inline_for_extraction
+val validate_t_at_most
+  (#base_t #len_t #pos_t: Type0)
+  {| inst: I.input_stream_inst base_t len_t pos_t  |}
+       (n:U32.t)
+       (#nz: _)
+       (#wk: _)
+       (#k:parser_kind nz wk)
+       (#t:Type)
+       (#p:parser k t)
+       (#extra_state: _)
+       (#ha:_)
+       (#use_error_handler:bool)
+       (v:validate_with_action_t #base_t #len_t #pos_t p extra_state ha use_error_handler)
+  : validate_with_action_t #base_t #len_t #pos_t (parse_t_at_most n p) extra_state ha use_error_handler
+
+noextract inline_for_extraction
+val validate_t_exact
+  (#base_t #len_t #pos_t: Type0)
+  {| inst: I.input_stream_inst base_t len_t pos_t  |}
+       (n:U32.t)
+       (#nz: _)
+       (#wk: _)
+       (#k:parser_kind nz wk)
+       (#t:Type)
+       (#p:parser k t)
+       (#extra_state: _)
+       (#ha:_)
+       (#use_error_handler:bool)
+       (v:validate_with_action_t #base_t #len_t #pos_t p extra_state ha use_error_handler)
+  : validate_with_action_t #base_t #len_t #pos_t (parse_t_exact n p) extra_state ha use_error_handler
+
+inline_for_extraction noextract
+val read_filter
+  (#base_t #len_t #pos_t: Type0)
+  {| inst: I.input_stream_inst base_t len_t pos_t  |}
+       (#nz:_)
+       (#k: parser_kind nz WeakKindStrongPrefix)
+       (#t: Type0)
+       (#p: parser k t)
+       (p32: leaf_reader #base_t #len_t #pos_t p)
+       (f: (t -> bool))
+    : leaf_reader #base_t #len_t #pos_t (parse_filter p f)
+
+inline_for_extraction noextract
+val read_impos
+  (#base_t #len_t #pos_t: Type0)
+  {| inst: I.input_stream_inst base_t len_t pos_t  |}
+    ()
+    : leaf_reader #base_t #len_t #pos_t (parse_impos())
+
+noextract
+inline_for_extraction
+val action_bind
+  (#base_t #len_t #pos_t: Type0)
+  {| inst: I.input_stream_inst base_t len_t pos_t  |}
+      (name: string)
+      (#extra_state: state_dict)
+      (#use_error_handler:bool)
+      (#a: Type)
+      (f: action #base_t #len_t #pos_t extra_state a use_error_handler)
+      (#b:Type) (g: (a -> action #base_t #len_t #pos_t extra_state b use_error_handler))
+: action #base_t #len_t #pos_t extra_state b use_error_handler
+
+noextract
+inline_for_extraction
+val action_weaken
+  (#base_t #len_t #pos_t: Type0)
+  {| inst: I.input_stream_inst base_t len_t pos_t  |}
+      (#d1: state_dict)
+      (#use_error_handler:bool)
+      (#a: Type)
+      (f: action #base_t #len_t #pos_t d1 a use_error_handler)
+      (d2: state_dict)
+      (d2_extends: squash (state_dict_weaken_prop d1 d2))
+: action #base_t #len_t #pos_t d2 a use_error_handler
+
+noextract
+inline_for_extraction
+val action_call
+  (#base_t #len_t #pos_t: Type0)
+  {| inst: I.input_stream_inst base_t len_t pos_t  |}
+      (#d': state_dict)
+      (#use_error_handler:bool)
+      (#a: Type)
+      (act: action #base_t #len_t #pos_t d' a use_error_handler)
+      (d: state_dict)
+      (#f: Ghost.erased ((x: refine_bool_t string d.state_p) -> Tot (option (refine_bool_t string d'.state_p)))) // TODO: change to GTot once we switch to ghost bijections
+      (#g: Ghost.erased (refine_bool_t string d'.state_p -> Tot (refine_bool_t string d.state_p)))
+      (sq: squash (state_dict_rename_prop d d' f g))
+: action #base_t #len_t #pos_t d a use_error_handler
+
+noextract
+inline_for_extraction
+val action_deref
+  (#base_t #len_t #pos_t: Type0)
+  {| inst: I.input_stream_inst base_t len_t pos_t  |}
+      (name: string)
+      (#a:Type0) (x:ref a) (#use_error_handler: bool)
+: action #base_t #len_t #pos_t (state_dict_singleton name (pts_to x #1.0R)) a use_error_handler
+
+noextract
+inline_for_extraction
+val action_assignment
+  (#base_t #len_t #pos_t: Type0)
+  {| inst: I.input_stream_inst base_t len_t pos_t  |}
+      (name: string)
+      (#a:Type) (x:ref a) (w: a) (#use_error_handler: bool)
+: action #base_t #len_t #pos_t (state_dict_singleton name (pts_to x #1.0R)) a use_error_handler
+
+noextract
+inline_for_extraction
+val action_return
+  (#base_t #len_t #pos_t: Type0)
+  {| inst: I.input_stream_inst base_t len_t pos_t  |}
+      (#extra_state: state_dict)
+      (#use_error_handler:bool)
+      (#a: Type)
+      (x: a)
+: action #base_t #len_t #pos_t extra_state a use_error_handler
+
+noextract
+inline_for_extraction
+val action_return_true
+  (#base_t #len_t #pos_t: Type0)
+  {| inst: I.input_stream_inst base_t len_t pos_t  |}
+      (#extra_state: state_dict)
+      (#use_error_handler:bool)
+: action #base_t #len_t #pos_t extra_state bool use_error_handler
+
+noextract
+inline_for_extraction
+val action_abort
+  (#base_t #len_t #pos_t: Type0)
+  {| inst: I.input_stream_inst base_t len_t pos_t  |}
+      (#extra_state: state_dict)
+      (#use_error_handler:bool)
+: action #base_t #len_t #pos_t extra_state bool use_error_handler
+
+noextract
+inline_for_extraction
+val action_seq
+  (#base_t #len_t #pos_t: Type0)
+  {| inst: I.input_stream_inst base_t len_t pos_t  |}
+      (#extra_state: state_dict)
+      (#use_error_handler:bool)
+      (#a: Type)
+      (f: action #base_t #len_t #pos_t extra_state a use_error_handler)
+      (#b: Type)
+      (g: action #base_t #len_t #pos_t extra_state b use_error_handler)
+: action #base_t #len_t #pos_t extra_state b use_error_handler
+
+noextract
+inline_for_extraction
+val action_ite
+  (#base_t #len_t #pos_t: Type0)
+  {| inst: I.input_stream_inst base_t len_t pos_t  |}
+      (#extra_state: state_dict)
+      (#use_error_handler:bool)
+      (#a: Type)
+      (guard: bool)
+      (then_: (squash (guard == true) -> action #base_t #len_t #pos_t extra_state a use_error_handler))
+      (else_: (squash (guard == false) -> action #base_t #len_t #pos_t extra_state a use_error_handler))
+: action #base_t #len_t #pos_t extra_state a use_error_handler
+
+inline_for_extraction noextract
+val validate_with_comment
+  (#base_t #len_t #pos_t: Type0)
+  {| inst: I.input_stream_inst base_t len_t pos_t  |}
+      (c: string)
+      (#nz:bool)
+      (#wk: _)
+      (#k:parser_kind nz wk)
+      (#t:Type)
+      (#p:parser k t)
+      (#extra_state: state_dict)
+      (#has_action:bool)
+      (#use_error_handler:bool)
+      (v: validate_with_action_t #base_t #len_t #pos_t p extra_state has_action use_error_handler)
+: validate_with_action_t #base_t #len_t #pos_t p extra_state has_action use_error_handler
+
+inline_for_extraction noextract
+val validate_unit
+  (#base_t #len_t #pos_t: Type0)
+  {| inst: I.input_stream_inst base_t len_t pos_t  |}
+      (#extra_state: state_dict)
+      (#use_error_handler:bool)
+: validate_with_action_t #base_t #len_t #pos_t parse_unit extra_state false use_error_handler
+
+inline_for_extraction noextract
+val validate_unit_refinement
+  (#base_t #len_t #pos_t: Type0)
+  {| inst: I.input_stream_inst base_t len_t pos_t  |}
+      (f: unit -> bool)
+      (cf: string)
+      (#extra_state: state_dict)
+      (#use_error_handler:bool)
+: validate_with_action_t #base_t #len_t #pos_t (parse_filter parse_unit f) extra_state false use_error_handler
+
+inline_for_extraction noextract
+val validate_dep_pair
+  (#base_t #len_t #pos_t: Type0)
+  {| inst: I.input_stream_inst base_t len_t pos_t  |}
+      (name1: string)
+      (#nz1:_)
+      (#k1:parser_kind nz1 WeakKindStrongPrefix)
+      (#t1:Type)
+      (#p1:parser k1 t1)
+      (#extra_state: state_dict)
+      (#has_action1:bool)
+      (#use_error_handler:bool)
+      (v1:validate_with_action_no_read #base_t #len_t #pos_t p1 extra_state has_action1 use_error_handler)
+      (r1: leaf_reader #base_t #len_t #pos_t p1)
+      (#nz2:_)
+      (#wk2: _)
+      (#k2:parser_kind nz2 wk2)
+      (#t2:t1 -> Type)
+      (#p2:(x:t1 -> parser k2 (t2 x)))
+      (#has_action2:bool)
+      (v2:(x:t1 -> validate_with_action_t #base_t #len_t #pos_t (p2 x) extra_state has_action2 use_error_handler))
+  : validate_with_action_t
+      #base_t #len_t #pos_t
+      (p1 `parse_dep_pair` p2)
+      extra_state
+      (has_action1 || has_action2)
+      use_error_handler
+
+inline_for_extraction noextract
+val validate_dep_pair_with_action
+  (#base_t #len_t #pos_t: Type0)
+  {| inst: I.input_stream_inst base_t len_t pos_t  |}
+      (#nz1:_)
+      (#k1:parser_kind nz1 WeakKindStrongPrefix)
+      (#t1:Type)
+      (#p1:parser k1 t1)
+      (#extra_state: state_dict)
+      (#has_action1:bool)
+      (#use_error_handler:bool)
+      (v1:validate_with_action_no_read #base_t #len_t #pos_t p1 extra_state has_action1 use_error_handler)
+      (r1: leaf_reader #base_t #len_t #pos_t p1)
+      (a:t1 -> action #base_t #len_t #pos_t extra_state bool use_error_handler)
+      (#nz2:_)
+      (#wk2: _)
+      (#k2:parser_kind nz2 wk2)
+      (#t2:t1 -> Type)
+      (#p2:(x:t1 -> parser k2 (t2 x)))
+      (#has_action2:bool)
+      (v2:(x:t1 -> validate_with_action_t #base_t #len_t #pos_t (p2 x) extra_state has_action2 use_error_handler))
+  : validate_with_action_t
+      #base_t #len_t #pos_t
+      (p1 `parse_dep_pair` p2)
+      extra_state
+      true
+      use_error_handler
+
+inline_for_extraction noextract
+val validate_dep_pair_with_refinement
+  (#base_t #len_t #pos_t: Type0)
+  {| inst: I.input_stream_inst base_t len_t pos_t  |}
+      (p1_is_constant_size_without_actions: bool)
+      (name1: string)
+      (#nz1:_)
+      (#k1:parser_kind nz1 WeakKindStrongPrefix)
+      (#t1:Type)
+      (#p1:parser k1 t1)
+      (#extra_state: state_dict)
+      (#has_action1:bool)
+      (#use_error_handler:bool)
+      (v1:validate_with_action_no_read #base_t #len_t #pos_t p1 extra_state has_action1 use_error_handler)
+      (r1: leaf_reader #base_t #len_t #pos_t p1)
+      (f: t1 -> bool)
+      (#nz2:_)
+      (#wk2: _)
+      (#k2:parser_kind nz2 wk2)
+      (#t2:refine _ f -> Type)
+      (#p2:(x:refine _ f -> parser k2 (t2 x)))
+      (#has_action2:bool)
+      (v2:(x:refine _ f -> validate_with_action_t #base_t #len_t #pos_t (p2 x) extra_state has_action2 use_error_handler))
+  : validate_with_action_t
+      #base_t #len_t #pos_t
+      ((p1 `parse_filter` f) `parse_dep_pair` p2)
+      extra_state
+      (has_action1 || has_action2)
+      use_error_handler
+
+inline_for_extraction noextract
+val validate_with_dep_action
+  (#base_t #len_t #pos_t: Type0)
+  {| inst: I.input_stream_inst base_t len_t pos_t  |}
+      (name: string)
+      (#nz:_)
+      (#k:parser_kind nz WeakKindStrongPrefix)
+      (#t:Type)
+      (#p:parser k t)
+      (#extra_state: state_dict)
+      (#has_action:bool)
+      (#use_error_handler:bool)
+      (v:validate_with_action_no_read #base_t #len_t #pos_t p extra_state has_action use_error_handler)
+      (r:leaf_reader #base_t #len_t #pos_t p)
+      (a: t -> action #base_t #len_t #pos_t extra_state bool use_error_handler)
+  : validate_with_action_t #base_t #len_t #pos_t p extra_state true use_error_handler
+
+inline_for_extraction noextract
+val validate____UINT8
+  (#base_t #len_t #pos_t: Type0)
+  {| inst: I.input_stream_inst base_t len_t pos_t  |}
+  (#extra_state: state_dict)
+  (#use_error_handler:bool)
+: validate_with_action_no_read #base_t #len_t #pos_t parse____UINT8 extra_state false use_error_handler
+
+inline_for_extraction noextract
+val read____UINT8
+  (#base_t #len_t #pos_t: Type0)
+  {| inst: I.input_stream_inst base_t len_t pos_t  |}
+: leaf_reader #base_t #len_t #pos_t parse____UINT8
+
+inline_for_extraction noextract
+val validate____UINT8BE
+  (#base_t #len_t #pos_t: Type0)
+  {| inst: I.input_stream_inst base_t len_t pos_t  |}
+  (#extra_state: state_dict)
+  (#use_error_handler:bool)
+: validate_with_action_no_read #base_t #len_t #pos_t parse____UINT8BE extra_state false use_error_handler
+
+inline_for_extraction noextract
+val read____UINT8BE
+  (#base_t #len_t #pos_t: Type0)
+  {| inst: I.input_stream_inst base_t len_t pos_t  |}
+: leaf_reader #base_t #len_t #pos_t parse____UINT8BE
+
+inline_for_extraction noextract
+val validate____UINT16BE
+  (#base_t #len_t #pos_t: Type0)
+  {| inst: I.input_stream_inst base_t len_t pos_t  |}
+  (#extra_state: state_dict)
+  (#use_error_handler:bool)
+: validate_with_action_no_read #base_t #len_t #pos_t parse____UINT16BE extra_state false use_error_handler
+
+inline_for_extraction noextract
+val read____UINT16BE
+  (#base_t #len_t #pos_t: Type0)
+  {| inst: I.input_stream_inst base_t len_t pos_t  |}
+: leaf_reader #base_t #len_t #pos_t parse____UINT16BE
+
+inline_for_extraction noextract
+val validate____UINT32BE
+  (#base_t #len_t #pos_t: Type0)
+  {| inst: I.input_stream_inst base_t len_t pos_t  |}
+  (#extra_state: state_dict)
+  (#use_error_handler:bool)
+: validate_with_action_no_read #base_t #len_t #pos_t parse____UINT32BE extra_state false use_error_handler
+
+inline_for_extraction noextract
+val read____UINT32BE
+  (#base_t #len_t #pos_t: Type0)
+  {| inst: I.input_stream_inst base_t len_t pos_t  |}
+: leaf_reader #base_t #len_t #pos_t parse____UINT32BE
+
+inline_for_extraction noextract
+val validate____UINT64BE
+  (#base_t #len_t #pos_t: Type0)
+  {| inst: I.input_stream_inst base_t len_t pos_t  |}
+  (#extra_state: state_dict)
+  (#use_error_handler:bool)
+: validate_with_action_no_read #base_t #len_t #pos_t parse____UINT64BE extra_state false use_error_handler
+
+inline_for_extraction noextract
+val read____UINT64BE
+  (#base_t #len_t #pos_t: Type0)
+  {| inst: I.input_stream_inst base_t len_t pos_t  |}
+: leaf_reader #base_t #len_t #pos_t parse____UINT64BE
+
+inline_for_extraction noextract
+val validate____UINT16
+  (#base_t #len_t #pos_t: Type0)
+  {| inst: I.input_stream_inst base_t len_t pos_t  |}
+  (#extra_state: state_dict)
+  (#use_error_handler:bool)
+: validate_with_action_no_read #base_t #len_t #pos_t parse____UINT16 extra_state false use_error_handler
+
+inline_for_extraction noextract
+val read____UINT16
+  (#base_t #len_t #pos_t: Type0)
+  {| inst: I.input_stream_inst base_t len_t pos_t  |}
+: leaf_reader #base_t #len_t #pos_t parse____UINT16
+
+inline_for_extraction noextract
+val validate____UINT32
+  (#base_t #len_t #pos_t: Type0)
+  {| inst: I.input_stream_inst base_t len_t pos_t  |}
+  (#extra_state: state_dict)
+  (#use_error_handler:bool)
+: validate_with_action_no_read #base_t #len_t #pos_t parse____UINT32 extra_state false use_error_handler
+
+inline_for_extraction noextract
+val read____UINT32
+  (#base_t #len_t #pos_t: Type0)
+  {| inst: I.input_stream_inst base_t len_t pos_t  |}
+: leaf_reader #base_t #len_t #pos_t parse____UINT32
+
+inline_for_extraction noextract
+val validate____UINT64
+  (#base_t #len_t #pos_t: Type0)
+  {| inst: I.input_stream_inst base_t len_t pos_t  |}
+  (#extra_state: state_dict)
+  (#use_error_handler:bool)
+: validate_with_action_no_read #base_t #len_t #pos_t parse____UINT64 extra_state false use_error_handler
+
+inline_for_extraction noextract
+val read____UINT64
+  (#base_t #len_t #pos_t: Type0)
+  {| inst: I.input_stream_inst base_t len_t pos_t  |}
+: leaf_reader #base_t #len_t #pos_t parse____UINT64
+
+inline_for_extraction noextract
+val read_unit
+  (#base_t #len_t #pos_t: Type0)
+  {| inst: I.input_stream_inst base_t len_t pos_t  |}
+: leaf_reader #base_t #len_t #pos_t (parse_ret ())
+
+inline_for_extraction noextract
+val validate_all_bytes
+  (#base_t #len_t #pos_t: Type0)
+  {| inst: I.input_stream_inst base_t len_t pos_t  |}
+  (#extra_state: state_dict)
+  (#use_error_handler:bool)
+: validate_with_action_t #base_t #len_t #pos_t parse_all_bytes extra_state false use_error_handler
+
+inline_for_extraction noextract
+val validate_drop
+  (#base_t #len_t #pos_t: Type0)
+  {| inst: I.input_stream_inst base_t len_t pos_t  |}
+      (#nz:bool)
+      (#wk: _)
+      (#k:parser_kind nz wk)
+      (#t:Type)
+      (#p:parser k t)
+      (#extra_state: state_dict)
+      (#has_action:bool)
+      (#use_error_handler:bool)
+      (v: validate_with_action_no_read #base_t #len_t #pos_t p extra_state has_action use_error_handler)
+: validate_with_action_t #base_t #len_t #pos_t p extra_state has_action use_error_handler
+
+inline_for_extraction noextract
+val validate_without_reading
+  (#base_t #len_t #pos_t: Type0)
+  {| inst: I.input_stream_inst base_t len_t pos_t  |}
+      (#nz:bool)
+      (#wk: _)
+      (#k:parser_kind nz wk)
+      (#t:Type)
+      (#p:parser k t)
+      (#extra_state: state_dict)
+      (#has_action:bool)
+      (#use_error_handler:bool)
+      (v: validate_with_action_no_read #base_t #len_t #pos_t p extra_state has_action use_error_handler)
+: validate_with_action_t #base_t #len_t #pos_t p extra_state has_action use_error_handler
+
+noextract
+inline_for_extraction
+val action_field_pos_64
+  (#base_t #len_t #pos_t: Type0)
+  {| inst: I.input_stream_inst base_t len_t pos_t  |}
+      (#extra_state: state_dict)
+      (#use_error_handler:bool)
+: action #base_t #len_t #pos_t extra_state U64.t use_error_handler
+
+noextract
+inline_for_extraction
+val action_field_pos_32
+  (#base_t #len_t #pos_t: Type0)
+  {| inst: I.input_stream_inst base_t len_t pos_t  |}
+      (#extra_state: state_dict)
+      (#use_error_handler:bool)
+: action #base_t #len_t #pos_t extra_state U32.t use_error_handler
+
+inline_for_extraction noextract
+let field_ptr_t
+  (base_t len_t pos_t: Type0)
+  {| inst: I.input_stream_inst base_t len_t pos_t  |}
+  (ptr_t: Type0)
+: Type0
+= (sl_base: base_t) ->
+  (sl_len: len_t) ->
+  (sl_pos: pos_t) ->
+  (contents_sl: Ghost.erased (Seq.seq U8.t)) ->
+  (v_sl: Ghost.erased (Seq.seq U8.t)) ->
+  stt ptr_t
+    (I.pts_to sl_base sl_len sl_pos contents_sl v_sl)
+    (fun _ -> I.pts_to sl_base sl_len sl_pos contents_sl v_sl)
+
+inline_for_extraction noextract
+let field_ptr_after_t
+  (base_t len_t pos_t: Type0)
+  {| inst: I.input_stream_inst base_t len_t pos_t  |}
+  (ptr_t: Type0)
+: Type0
+= (sz: U64.t) ->
+  (write_to: ref ptr_t) ->
+  (sl_base: base_t) ->
+  (sl_len: len_t) ->
+  (sl_pos: pos_t) ->
+  (w: Ghost.erased ptr_t) ->
+  (contents_sl: Ghost.erased (Seq.seq U8.t)) ->
+  (v_sl: Ghost.erased (Seq.seq U8.t)) ->
+  stt bool
+    (pts_to write_to #1.0R w ** I.pts_to sl_base sl_len sl_pos contents_sl v_sl)
+    (fun _ -> exists* w' . pts_to write_to #1.0R w' ** I.pts_to sl_base sl_len sl_pos contents_sl v_sl)
+
+noextract
+inline_for_extraction
+val action_field_ptr
+  (#base_t #len_t #pos_t: Type0)
+  {| inst: I.input_stream_inst base_t len_t pos_t  |}
+      (#ptr_t: Type0)
+      (f: option (field_ptr_t base_t len_t pos_t ptr_t))
+      (sq: squash (Some? f))
+      (#extra_state: state_dict)
+      (#use_error_handler:bool)
+: action #base_t #len_t #pos_t extra_state ptr_t use_error_handler
+
+noextract
+inline_for_extraction
+val action_field_ptr_after
+  (#base_t #len_t #pos_t: Type0)
+  {| inst: I.input_stream_inst base_t len_t pos_t  |}
+      (#ptr_t: Type0)
+      (f: option (field_ptr_after_t base_t len_t pos_t ptr_t))
+      (sq: squash (Some? f))
+      (name: string)
+      (sz: U64.t)
+      (write_to: ref ptr_t)
+      (#use_error_handler:bool)
+: action #base_t #len_t #pos_t (state_dict_singleton name (pts_to write_to #1.0R)) bool use_error_handler
+
+inline_for_extraction noextract
+val validate_all_zeros
+  (#base_t #len_t #pos_t: Type0)
+  {| inst: I.input_stream_inst base_t len_t pos_t  |}
+  (#extra_state: state_dict)
+  (#use_error_handler:bool)
+: validate_with_action_t #base_t #len_t #pos_t parse_all_zeros extra_state false use_error_handler
+
+inline_for_extraction noextract
+val validate_string
+  (#base_t #len_t #pos_t: Type0)
+  {| inst: I.input_stream_inst base_t len_t pos_t  |}
+      (#k: parser_kind true WeakKindStrongPrefix)
+      (#t: eqtype)
+      (#p: parser k t)
+      (#extra_state: state_dict)
+      (#ha:bool)
+      (#use_error_handler:bool)
+      (v: validate_with_action_no_read #base_t #len_t #pos_t p extra_state ha use_error_handler)
+      (r: leaf_reader #base_t #len_t #pos_t p)
+      (terminator: t)
+: validate_with_action_t #base_t #len_t #pos_t (parse_string p terminator) extra_state ha use_error_handler
+
+inline_for_extraction noextract
+val validate_nlist_constant_size_without_actions
+  (#base_t #len_t #pos_t: Type0)
+  {| inst: I.input_stream_inst base_t len_t pos_t  |}
+      (n:U32.t)
+      (n_is_const:option nat { memoizes_n_as_const n_is_const n})
+      (payload_is_constant_size: bool)
+      (#wk: _)
+      (#k:parser_kind true wk)
+      (#t:Type)
+      (#p:parser k t)
+      (#extra_state: state_dict)
+      (#use_error_handler:bool)
+      (v: validate_with_action_t #base_t #len_t #pos_t p extra_state false use_error_handler)
+: validate_with_action_t #base_t #len_t #pos_t (parse_nlist n n_is_const p) extra_state false use_error_handler
